src/impl/TLS13.Impl.Client.Driver.Receive.fsti
@@ -6,11 +6,14 @@ open Pulse.Lib.Pervasives
 open Pulse.Lib.Array.PtsTo
 
 module B = TLS13.Bytes
+module CI = Common.ChannelImplementation
 module CR = TLS13.Impl.ConnectionState.Repr
 module CS = TLS13.Spec.StateMachine
 module CT = TLS13.Impl.Client.Types
 module DS = TLS13.Impl.Client.Driver.State
+module L = TLS13.Impl.Messages
 module SZ = FStar.SizeT
+module TChannel = TLS13.Impl.Channel
 module U16 = FStar.UInt16
 module U8 = FStar.UInt8
 open TLS13.Impl.Client.Driver.State
@@ -23,7 +26,8 @@ fn run
   (fuel:SZ.t)
   requires client_driver_connected d 'st0 'received0 'sent0 **
            pts_to out 'old_out **
-           pure (B.length 'old_out == SZ.v out_len)
+           pure (B.length 'old_out == SZ.v out_len /\
+                 L.max_record_fragment_len <= SZ.v out_len)
   returns result:client_receive_result
   ensures exists* st1 received1 sent1 out_bytes.
           client_driver_connected d st1 received1 sent1 **
@@ -38,6 +42,16 @@ fn run
                   (Ghost.reveal 'received0) /\
                 client_driver_sent_log_exact st1 sent1 /\
                 client_driver_received_log_accounted st1 received1 /\
+                TChannel.application_log st1 ==
+                  (if result.DS.client_receive_status == DriverWorkflowOk
+                   then
+                     CI.append_received
+                       (TChannel.application_log 'st0)
+                       (FStar.Seq.slice
+                         out_bytes
+                         0
+                         (SZ.v result.DS.client_receive_len))
+                   else TChannel.application_log 'st0) /\
                 (exists obs app_out.
                   client_driver_receive_correct
                     'st0
